litform

Foundation/AutoProver/Litform.lean
@@ -1,9 +1,108 @@
 import Foundation.Logic.Calculus
+import Foundation.Logic.HilbertStyle.Supplemental
 import Foundation.Vorspiel.Meta
+import Mathlib.Tactic.TryThis
+import Mathlib.Util.AtomM
+import Foundation.Propositional.Hilbert.WellKnown
 
-open Qq Lean Elab Meta Tactic
+inductive DbgResult (α : Type u) : α → Type u
+  | intro : (a b : α) → a = b → DbgResult α a
 
-namespace LO
+instance {α} (a : α) : ToString (DbgResult α a) := ⟨fun r =>
+  match r with
+  | DbgResult.intro _ _ _ => "🎉 Proof Success! 🎉"⟩
+
+namespace Qq
+
+open Mathlib Qq Lean Elab Meta Tactic
+
+def rflQ {α : Q(Sort u)} (a : Q($α)) : Q($a = $a) := q(rfl)
+
+def toQList {α : Q(Type u)} : List Q($α) → Q(List $α)
+  |     [] => q([])
+  | a :: v => q($a :: $(toQList v))
+
+lemma List.mem_of_eq {a b : α} {l} (h : a = b) : a ∈ b :: l := by simp [h]
+
+lemma List.mem_of_mem {a b : α} {l : List α} (h : a ∈ l) : a ∈ b :: l := by simp [h]
+
+lemma List.mem_singleton_of_eq (a b : α) (h : a = b) : a ∈ [b] := by simp [h]
+
+def memQList? {α : Q(Type u)} (a : Q($α)) : (l : List Q($α)) → MetaM <| Option Q($a ∈ $(toQList l))
+  |     [] => return none
+  | b :: l => do
+      if (← isDefEq (← whnf a) (← whnf b)) then
+        let e : Q($a = $b) := rflQ a
+        return some q(List.mem_of_eq $e)
+      else
+        let some h ← memQList? a l | return none
+        return some q(List.mem_of_mem $h)
+
+def memQList?' (a : Expr) (l : List Expr) : MetaM (Option Expr) := do
+  let ⟨u, _, a⟩ ← inferTypeQ' a
+  memQList? (u := u) a l
+
+partial def ofQList {α : Q(Type u)} (l : Q(List $α)) : MetaM <| List Q($α) := do
+  match l with
+  |       ~q([]) => return []
+  | ~q($a :: $l) => return a :: (← ofQList l)
+
+end Qq
+
+namespace LO.Entailment
+
+variable {F : Type*} [LogicalConnective F] [DecidableEq F] {S : Type*} [Entailment F S]
+
+variable (𝓢 : S)
+
+abbrev TwoSided (Γ Δ : List F) : Prop := Γ ⊢[𝓢]! Δ.disj
+
+namespace TwoSided
+
+open FiniteContext
+
+variable {𝓢} [Entailment.Cl 𝓢]
+
+local notation Γ:45 " ⟹ " Δ:46 => TwoSided 𝓢 Γ Δ
+
+lemma provable_of (h : [] ⟹ [φ]) : 𝓢 ⊢! φ :=
+  FiniteContext.provable_iff_provable.mpr <| left_Disj!_intro [φ] (by simp) ⨀! h
+
+lemma weakening (h : Γ₁ ⟹ Δ₁) (HΓ : Γ₁ ⊆ Γ₂ := by simp) (HΔ : Δ₁ ⊆ Δ₂ := by simp) : Γ₂ ⟹ Δ₂ :=
+  FiniteContext.weakening! HΓ <| left_Disj!_intro Δ₁ (fun _ hψ ↦ right_Disj!_intro _ (HΔ hψ)) ⨀! h
+
+lemma rotate (hφ : Γ ⟹ Δ ++ [φ]) : Γ ⟹ φ :: Δ := weakening hφ
+
+lemma and_right (Γ Δ φ ψ) (hφ : Γ ⟹ φ :: Δ) (hψ : Γ ⟹ ψ :: Δ) : Γ ⟹ φ ⋏ ψ :: Δ := by
+  have : Γ ⊢[𝓢]! (φ :: Δ).disj ➝ (ψ :: Δ).disj ➝ (φ ⋏ ψ :: Δ).disj := by
+    apply left_Disj!_intro
+    rintro χ hχ
+    rcases show χ = φ ∨ χ ∈ Δ by simpa using hχ with (rfl | hχ)
+    · apply deduct!
+      apply left_Disj!_intro
+      intro ξ hξ
+      rcases show ξ = ψ ∨ ξ ∈ Δ by simpa using hξ with (rfl | hξ)
+      · apply deduct!
+        apply right_Disj!_intro (χ ⋏ ξ :: Δ) (φ := χ ⋏ ξ) List.mem_cons_self ⨀! (K!_intro by_axm₁! by_axm₀!)
+      · apply right_Disj!_intro _ (by simp [hξ])
+    · apply deduct!
+      apply dhyp!
+      apply right_Disj!_intro _ (φ := χ) (by simp [hχ]) ⨀! by_axm₀!
+  exact this ⨀! hφ ⨀! hψ
+
+variable (𝓢)
+
+lemma right_closed (Γ φ Δ) (h : φ ∈ Γ) : Γ ⟹ φ :: Δ := right_Disj!_intro _ (φ := φ) (by simp) ⨀! (by_axm! h)
+
+lemma left_closed (Γ φ Δ) (h : φ ∈ Δ) : (φ :: Γ) ⟹ Δ := right_Disj!_intro _ (φ := φ) h ⨀! by_axm!
+
+end TwoSided
+
+end LO.Entailment
+
+namespace LO.Meta
+
+open Mathlib Qq Lean Elab Meta Tactic
 
 inductive Litform (α : Type*) : Type _
   | atom (a : α)  : Litform α
@@ -13,6 +112,7 @@ inductive Litform (α : Type*) : Type _
   | or            : Litform α → Litform α → Litform α
   | neg           : Litform α → Litform α
   | imply         : Litform α → Litform α → Litform α
+  | iff           : Litform α → Litform α → Litform α
 
 namespace Litform
 
@@ -29,13 +129,14 @@ section ToString
 variable [ToString α]
 
 def toStr : Litform α → String
-  | ⊤      => "⊤"
-  | ⊥      => "⊥"
-  | atom a => toString a
-  | ∼φ     => "(¬" ++ toStr φ ++ ")"
-  | φ ⋏ ψ  => "(" ++ toStr φ ++ " ∧ " ++ toStr ψ ++ ")"
-  | φ ⋎ ψ  => "(" ++ toStr φ ++ " ∨ "  ++ toStr ψ ++ ")"
-  | φ ➝ ψ => "(" ++ toStr φ ++ " ➝ "  ++ toStr ψ ++ ")"
+  |       ⊤ => "⊤"
+  |       ⊥ => "⊥"
+  |  atom a => s!"atom {toString a}"
+  |      ∼φ => "(¬" ++ toStr φ ++ ")"
+  |   φ ⋏ ψ => "(" ++ toStr φ ++ " ∧ " ++ toStr ψ ++ ")"
+  |   φ ⋎ ψ => "(" ++ toStr φ ++ " ∨ "  ++ toStr ψ ++ ")"
+  |   φ ➝ ψ => "(" ++ toStr φ ++ " → "  ++ toStr ψ ++ ")"
+  | iff φ ψ => "(" ++ toStr φ ++ " ↔ "  ++ toStr ψ ++ ")"
 
 instance : Repr (Litform α) := ⟨fun t _ => toStr t⟩
 
@@ -43,41 +144,146 @@ instance : ToString (Litform α) := ⟨toStr⟩
 
 end ToString
 
-namespace Meta
-
 variable (F : Q(Type*)) (ls : Q(LogicalConnective $F))
 
-abbrev Lit (F : Q(Type*)) := Litform Q($F)
+abbrev _root_.LO.Meta.Lit := Litform Expr
 
-abbrev toExpr : Lit F → Q($F)
-  | atom e  => ψ($e)
-  | ⊤       => ψ(⊤)
-  | ⊥       => ψ(⊥)
-  | φ ⋏ ψ   => ψ($(toExpr φ) ⋏ $(toExpr ψ))
-  | φ ⋎ ψ   => ψ($(toExpr φ) ⋎ $(toExpr ψ))
-  | ∼φ      => ψ(∼$(toExpr φ))
-  | φ ➝ ψ  => ψ($(toExpr φ) ➝ $(toExpr ψ))
+variable {F}
 
-partial def denote : Q($F) → MetaM (Lit F)
-  | ∼ψ(⊤)        => return ⊤
-  | ∼ψ(⊥)        => return ⊥
-  | ∼ψ($φ ⋏ $ψ)  => return (←denote φ) ⋏ (←denote ψ)
-  | ∼ψ($φ ⋎ $ψ)  => return (←denote φ) ⋎ (←denote ψ)
-  | ∼ψ($φ ➝ $ψ) => return (←denote φ) ➝ (←denote ψ)
-  | ∼ψ($φ ⭤ $ψ)  => return (←denote φ) ⭤ (←denote ψ)
-  | ∼ψ(∼$φ)      => return ∼(←denote φ)
-  | ∼ψ($e)       => return atom e
+abbrev toExpr : Lit → Q($F)
+  |  atom e => e
+  |       ⊤ => q(⊤)
+  |       ⊥ => q(⊥)
+  |   φ ⋏ ψ => q($(toExpr φ) ⋏ $(toExpr ψ))
+  |   φ ⋎ ψ => q($(toExpr φ) ⋎ $(toExpr ψ))
+  |      ∼φ => q(∼$(toExpr φ))
+  |   φ ➝ ψ => q($(toExpr φ) ➝ $(toExpr ψ))
+  | iff φ ψ => q($(toExpr φ) ⭤ $(toExpr ψ))
 
-instance denotation : Denotation ψ($F) (Lit F) where
-  denote' := denote F ls
-  toExpr' := toExpr F ls
+partial def summands {α : Q(Type $u)} (inst : Q(Add $α)) :
+    Q($α) → MetaM (List Q($α))
+  | ~q($x + $y) => return (← summands inst x) ++ (← summands inst y)
+  | n => return [n]
 
-abbrev DEq (φ ψ : Lit F) :=
-  letI := denotation F ls
-  Denotation.DEq F φ ψ
+partial def denote : Q($F) → MetaM Lit
+  |       ~q(⊤) => return ⊤
+  |       ~q(⊥) => return ⊥
+  | ~q($φ ⋏ $ψ) => return (←denote φ) ⋏ (←denote ψ)
+  | ~q($φ ⋎ $ψ) => return (←denote φ) ⋎ (←denote ψ)
+  | ~q($φ ➝ $ψ) => return (←denote φ) ➝ (←denote ψ)
+  | ~q($φ ⭤ $ψ) => return iff (←denote φ) (←denote ψ)
+  |     ~q(∼$φ) => return ∼(←denote φ)
+  |      ~q($e) => return atom e
 
-end Meta
+variable (F)
 
 end Litform
 
-end LO
+namespace CLProver
+
+initialize registerTraceClass `cl_prover
+initialize registerTraceClass `cl_prover.detail
+
+syntax (name := cl_prover) "cl_prover" : tactic
+
+structure Context where
+  levelF : Level
+  levelS : Level
+  levelE : Level
+  F : Q(Type levelF)
+  LC : Q(LogicalConnective $F)
+  DC : Q(DecidableEq $F)
+  S : Q(Type levelS)
+  E : Q(Entailment.{_, _, levelE} $F $S)
+  𝓢 : Q($S)
+  CL : Q(Entailment.Cl $𝓢)
+
+/-- The monad for `cl_prover` contains. -/
+abbrev M := ReaderT Context AtomM
+
+#check Entailment.TwoSided.right_closed
+/-- Apply the function
+  `n : ∀ {F} [LogicalConnective F] [DecidableEq F] {S} [Entailment F S] {𝓢} [Entailment.Cl 𝓢], _` to the
+implicit parameters in the context, and the given list of arguments. -/
+def Context.app (c : Context) (n : Name) : Array Expr → Expr :=
+  mkAppN <| @Expr.const n [c.levelF, c.levelS, c.levelE]
+    |>.app c.F |>.app c.LC |>.app c.DC |>.app c.S |>.app c.E |>.app c.𝓢 |>.app c.CL
+
+def iapp (n : Name) (xs : Array Expr) : M Expr := do
+  let c ← read
+  return c.app n xs
+
+def getGoalTwoSided (e : Q(Prop)) : MetaM ((c : Context) × List Q($c.F) × List Q($c.F)) := do
+  let ~q(@Entailment.TwoSided $F $LC $S $E $𝓢 $p $q) := e | throwError m!"(getGoal) error: {e} not a form of _ ⊢! _"
+  let .some DC ← trySynthInstanceQ q(DecidableEq $F)
+    | throwError m! "error: failed to find instance DecidableEq {F}"
+  let .some CL ← trySynthInstanceQ q(Entailment.Cl $𝓢)
+    | throwError m! "error: failed to find instance Entailment.Cl {𝓢}"
+  let Γ ← Qq.ofQList p
+  let Δ ← Qq.ofQList q
+  return ⟨⟨_, _, _, F, LC, DC, S, E, 𝓢, CL⟩, Γ, Δ⟩
+
+abbrev Sequent := List Lit
+
+def Lit.toExpr (φ : Lit) : M Expr := do
+  let c ← read
+  return Litform.toExpr c.LC φ
+
+def Sequent.toExprList (Γ : Sequent) : M (List Expr) := do
+  let c ← read
+  return Γ.map (Litform.toExpr c.LC)
+
+def Sequent.toExpr (Γ : Sequent) : M Expr := do
+  let c ← read
+  return toQList <| Γ.map (Litform.toExpr c.LC)
+
+def code (Γ Δ : Sequent) : M Expr := do
+  match Δ with
+  |     [] => throwError m!"mssg: {Γ} ⟹ {Δ} found"
+  | φ :: Δ =>
+    logInfo m!"case: {φ} :: {Δ}"
+    match ← memQList?' (← Lit.toExpr φ) (← Γ.toExprList) with
+    | .none => throwError m! "FAILED: {φ} ∉ {Γ}"
+    | .some e => do
+      let eΔ ← Sequent.toExpr Δ
+      let eΓ ← Sequent.toExpr Γ
+      let eφ ← Lit.toExpr φ
+      logInfo m!"e : {e}"
+      let k ← iapp ``LO.Entailment.TwoSided.right_closed #[eΓ, eφ, eΔ, e]
+      logInfo m!"k : {k}"
+      iapp ``LO.Entailment.TwoSided.right_closed #[eΓ, eφ, eΔ, e]
+
+
+elab "test2s" : tactic => withMainContext do
+  let ⟨c, L, R⟩ ← getGoalTwoSided <| ← whnfR <| ← getMainTarget
+  let Γ ← L.mapM (m := MetaM) (Litform.denote c.LC)
+  let Δ ← R.mapM (m := MetaM) (Litform.denote c.LC)
+  logInfo m!"{Γ} ⟹ {Δ}"
+  closeMainGoal `cl_prover <| ← AtomM.run .reducible <| ReaderT.run (code Γ Δ) c
+
+section
+
+section
+
+variable {F : Type*} [DecidableEq F] {S : Type*} [LogicalConnective F] [Entailment F S]
+
+variable {𝓢 : S} [Entailment.Cl 𝓢] {φ ψ : F}
+
+example : Entailment.TwoSided 𝓢 [φ ⋏ ⊤, ψ] [ψ, φ] := by { test2s }
+
+end
+section
+
+open LO.Propositional
+
+variable {φ ψ χ : Formula ℕ}
+
+example : Entailment.TwoSided Hilbert.Cl [φ ⋏ ⊤, ψ] [ψ, φ, .atom 9] := by { test2s }
+
+end
+
+end
+
+end CLProver
+
+end LO.Meta
